reflection: TermEq: start working on termination, pretty hairy

ulib/FStar.Reflection.TermEq.fst
@@ -5,24 +5,47 @@ open FStar.Reflection.Data
 open FStar.Reflection.Builtins
 module L = FStar.List.Tot
 
-let rec allP #a (pred : a -> Type0) (l : list a) : Type0 =
+let rec allP0 #a (pred : a -> Type0) (l : list a) : Type0 =
   match l with
   | [] -> True
-  | x::xs -> pred x /\ allP pred xs
+  | x::xs -> pred x /\ allP0 pred xs
+
+let rec allP #a #b (top:b) (pred : (x:a{x << top}) -> Type0) (l : list a{l << top}) : Type0 =
+  match l with
+  | [] -> True
+  | x::xs -> pred x /\ allP top pred xs
 
 let optP #a (pred : a -> Type0) (o : option a) : Type0 =
   match o with
   | None -> True
   | Some x -> pred x
 
-let rec memP_allP #a (pred : a -> Type) (x : a) (l : list a)
-  : Lemma (requires allP pred l /\ L.memP x l)
-          (ensures pred x)
-          [SMTPat (allP pred l); SMTPat (L.memP x l)]
+let rec memP_allP #a #b (top:b) (pred : (x:a{x << top}) -> Type) (x : a) (l : list a{l << top})
+  : Lemma (requires allP top pred l /\ L.memP x l)
+          (ensures x << top /\ pred x)
+          [SMTPat (allP top pred l); SMTPat (L.memP x l)]
   = match l with
     | [] -> ()
     | y::ys ->
-      if StrongExcludedMiddle.strong_excluded_middle (x == y) then () else memP_allP pred x ys
+      if StrongExcludedMiddle.strong_excluded_middle (x == y) then () else memP_allP top pred x ys
+
+let rec memP_allP0 #a (pred : a -> Type) (x : a) (l : list a)
+  : Lemma (requires allP0 pred l /\ L.memP x l)
+          (ensures pred x)
+          [SMTPat (allP0 pred l); SMTPat (L.memP x l)]
+  = match l with
+    | [] -> ()
+    | y::ys ->
+      if StrongExcludedMiddle.strong_excluded_middle (x == y) then () else memP_allP0 pred x ys
+
+let rec memP_dec #a (x : a) (l : list a)
+  : Lemma (requires L.memP x l)
+          (ensures x << l)
+          [SMTPat (L.memP x l)]
+  = match l with
+    | [] -> ()
+    | y::ys ->
+      if StrongExcludedMiddle.strong_excluded_middle (x == y) then () else memP_dec x ys
 
 type _cmpres =
   | Eq
@@ -92,14 +115,28 @@ let rec list_eq #a cmp l1 l2 =
   | _ -> Neq
 
 val list_dec_eq :
-#a:Type u#aa -> l1:(list a) -> l2:(list a) ->
-  f:(x:a{x << l1} -> y:a{y << l2} -> cmpres x y) ->
+#a:Type u#aa -> #b:Type u#bb -> top1:b -> top2:b ->
+  f:(x:a{x << top1} -> y:a{y << top2} -> cmpres x y) ->
+  l1:(list a){l1 << top1} -> l2:(list a){l2 << top2} ->
   cmpres l1 l2
-let rec list_dec_eq #a l1 l2 cmp =
+let rec list_dec_eq #a top1 top2 cmp l1 l2 =
   match l1, l2 with
   | [], [] -> Eq
   | x::xs, y::ys ->
-    cmp x y &&& list_dec_eq xs ys cmp
+    cmp x y &&& list_dec_eq top1 top2 cmp xs ys
+  | _ -> Neq
+
+(* Refinements shaped differently *)
+val list_dec_eq2 :
+#a:Type u#aa -> #b:Type u#bb -> top1:b -> top2:b ->
+  f:(x:a -> y:a{x << top1 /\ y << top2} -> cmpres x y) ->
+  l1:(list a){l1 << top1} -> l2:(list a){l2 << top2} ->
+  cmpres l1 l2
+let rec list_dec_eq2 #a top1 top2 cmp l1 l2 =
+  match l1, l2 with
+  | [], [] -> Eq
+  | x::xs, y::ys ->
+    cmp x y &&& list_dec_eq2 top1 top2 cmp xs ys
   | _ -> Neq
 
 val eq_eq : #a:eqtype -> comparator_for a
@@ -116,20 +153,17 @@ let ident_eq i1 i2 =
   eq_eq (fst i1) (fst i2)
 
 val univ_eq         : comparator_for universe
-val univ_view_eq    : comparator_for universe_view
 
-[@@admit_termination]
 let rec univ_eq (u1 u2 : universe) : cmpres u1 u2 =
   pack_inspect_universe u1;
   pack_inspect_universe u2;
   let uv1 = inspect_universe u1 in
   let uv2 = inspect_universe u2 in
-  univ_view_eq uv1 uv2
-and univ_view_eq (uv1 uv2 : universe_view) : cmpres uv1 uv2 =
   match uv1, uv2 with
   | Uv_Zero, Uv_Zero -> Eq
   | Uv_Succ u1, Uv_Succ u2 -> univ_eq u1 u2
-  | Uv_Max us1, Uv_Max us2 -> list_eq univ_eq us1 us2
+  | Uv_Max us1, Uv_Max us2 ->
+    list_dec_eq2 u1 u2 univ_eq us1 us2
   | Uv_BVar v1, Uv_BVar v2 -> eq_eq v1 v2
   | Uv_Name n1, Uv_Name n2 -> ident_eq n1 n2
   | Uv_Unif u1, Uv_Unif u2 -> Unknown
@@ -154,13 +188,9 @@ let const_eq c1 c2 =
 val ctxu_eq : comparator_for ctx_uvar_and_subst
 let ctxu_eq _ _ = Unknown
 
-(* supported term views *)
-let term_view_supp = tv:term_view{~(Tv_Unsupp? tv)}
-
 val term_eq         : comparator_for term
 val binder_eq       : comparator_for binder
 val aqual_eq        : comparator_for aqualv
-val term_view_eq    : comparator_for term_view_supp
 val arg_eq          : comparator_for argv
 val binding_bv_eq   : comparator_for bv
 val comp_eq         : comparator_for comp
@@ -178,15 +208,11 @@ let rec term_eq t1 t2 =
   match tv1, tv2 with
   | Tv_Unsupp, _
   | _, Tv_Unsupp -> Unknown
-  | _ -> term_view_eq tv1 tv2
-
-and term_view_eq (tv1 tv2 : term_view_supp) =
-  match tv1, tv2 with
   | Tv_Var v1, Tv_Var v2 -> bv_eq v1 v2
   | Tv_BVar v1, Tv_BVar v2 -> bv_eq v1 v2
   | Tv_FVar f1, Tv_FVar f2 -> fv_eq f1 f2
   | Tv_UInst f1 u1, Tv_UInst f2 u2 ->
-    fv_eq f1 f2 &&& list_eq univ_eq u1 u2
+    fv_eq f1 f2 &&& list_dec_eq2 t1 t2 univ_eq u1 u2
 
   | Tv_App h1 a1, Tv_App h2 a2 ->
     term_eq h1 h2 &&& arg_eq a1 a2
@@ -331,8 +357,16 @@ let rec defined_list #a (f : comparator_for a) (l1 l2 : list a)
     | x::xs, y::ys -> defined_list f xs ys
     | _ -> ()
 
+let rec defined_list_dec #a #b (t1 t2 : b) (f : comparator_for a)
+  (l1 : list a{l1 << t1})
+  (l2 : list a{l2 << t2})
+  : Lemma (requires (def2 f l1 l2)) (ensures defined (list_dec_eq2 t1 t2 f l1 l2))
+  = match l1, l2 with
+    | [], [] -> ()
+    | x::xs, y::ys -> defined_list_dec t1 t2 f xs ys
+    | _ -> ()
+
 val faithful_univ : universe -> Type0
-[@@admit_termination]
 let rec faithful_univ (u : universe) =
   match inspect_universe u with
   | Uv_Unif _ -> False (* We just forbid this *)
@@ -343,27 +377,27 @@ let rec faithful_univ (u : universe) =
   | Uv_Name _ -> True
 
   | Uv_Succ u -> faithful_univ u
-  | Uv_Max us -> allP faithful_univ us
+  | Uv_Max us -> allP u faithful_univ us
 
 val univ_faithful_lemma (u1 u2 : universe) : Lemma (requires faithful_univ u1 /\ faithful_univ u2) (ensures defined (univ_eq u1 u2))
-[@@admit_termination]
 let rec univ_faithful_lemma (u1 u2 : universe) =
   match inspect_universe u1, inspect_universe u2 with
   | Uv_Zero, Uv_Zero -> ()
   | Uv_Succ u1, Uv_Succ u2 -> univ_faithful_lemma u1 u2
   | Uv_Max us1, Uv_Max us2 ->
-    assert_norm (faithful_univ u1 <==> allP faithful_univ us1); // #2908
-    assert_norm (faithful_univ u2 <==> allP faithful_univ us2); // #2908
-    univ_faithful_lemma_list us1 us2;
-    assert_norm (univ_eq u1 u2 == list_eq univ_eq us1 us2); // #2908
+    assert_norm (faithful_univ u1 <==> allP u1 faithful_univ us1); // #2908
+    assert_norm (faithful_univ u2 <==> allP u2 faithful_univ us2); // #2908
+    univ_faithful_lemma_list u1 u2 us1 us2;
+    assert_norm (univ_eq u1 u2 == list_dec_eq2 u1 u2 univ_eq us1 us2); // #2908
     ()
   | Uv_BVar _, Uv_BVar _ -> ()
   | Uv_Name _, Uv_Name _ -> ()
   | _ -> ()
 
-and univ_faithful_lemma_list (us1 us2 : list universe)
-  : Lemma (requires allP faithful_univ us1 /\ allP faithful_univ us2)
-          (ensures defined (list_eq univ_eq us1 us2))
+and univ_faithful_lemma_list #b (u1 u2 : b) (us1 : list universe{us1 << u1}) (us2 : list universe{us2 << u2})
+  : Lemma (requires allP u1 faithful_univ us1 /\ allP u2 faithful_univ us2)
+          (ensures defined (list_dec_eq2 u1 u2 univ_eq us1 us2))
+          (decreases us1)
   =
     introduce forall x y. L.memP x us1 /\ L.memP y us2 ==> defined (univ_eq x y) with
      (introduce forall y. L.memP x us1 /\ L.memP y us2 ==> defined (univ_eq x y) with
@@ -373,7 +407,7 @@ and univ_faithful_lemma_list (us1 us2 : list universe)
       )
      )
     ;
-    defined_list univ_eq us1 us2
+    defined_list_dec u1 u2 univ_eq us1 us2
 
 val faithful : term -> Type0
 [@@admit_termination]
@@ -386,7 +420,7 @@ let rec faithful t =
   | Tv_Const _ -> True
 
   | Tv_UInst f us ->
-    allP faithful_univ us
+    allP t faithful_univ us
 
   | Tv_Unsupp -> False
   | Tv_App h a ->
@@ -411,7 +445,7 @@ let rec faithful t =
   | Tv_Match sc o brs ->
     faithful sc
      /\ None? o // stopgap
-     /\ allP faithful_branch brs
+     /\ allP0 faithful_branch brs
 
   | Tv_AscribedT e t tacopt eq ->
     faithful e
@@ -445,8 +479,8 @@ and faithful_pattern (p : pattern) : Type0 =
   match p with
   | Pat_Constant _ -> True
   | Pat_Cons h usopt pats ->
-    optP (allP faithful_univ) usopt
-     /\ allP faithful_pattern_arg pats
+    optP (allP0 faithful_univ) usopt
+     /\ allP0 faithful_pattern_arg pats
   (* non-binding bvs are always OK *)
   | Pat_Var bv _ -> True
   | Pat_Dot_Term None -> True
@@ -455,7 +489,7 @@ and faithful_pattern (p : pattern) : Type0 =
 and faithful_pattern_arg (pb : pattern * bool) =
   faithful_pattern (fst pb)
 
-and faithful_attrs ats = allP faithful ats
+and faithful_attrs ats = allP0 faithful ats
 
 and faithful_comp c =
   match inspect_comp c with
@@ -463,14 +497,14 @@ and faithful_comp c =
   | C_GTotal t -> faithful t
   | C_Lemma pre post pats -> faithful pre /\ faithful post /\ faithful pats
   | C_Eff us ef r args decs ->
-    allP faithful_univ us
+    allP0 faithful_univ us
      /\ faithful r
-     /\ allP faithful_arg args
-     /\ allP faithful decs
+     /\ allP0 faithful_arg args
+     /\ allP0 faithful decs
 
 val faithful_lemma (t1:term) (t2:term) : Lemma (requires faithful t1 /\ faithful t2) (ensures defined (term_eq t1 t2))
 
-#push-options "--z3rlimit 20"
+#push-options "--z3rlimit 40"
 
 [@@admit_termination]
 let rec faithful_lemma (t1 t2 : term) =
@@ -479,7 +513,16 @@ let rec faithful_lemma (t1 t2 : term) =
   | Tv_BVar _, Tv_BVar _
   | Tv_FVar _, Tv_FVar _ -> ()
   | Tv_UInst f1 us1, Tv_UInst f2 us2 ->
-    univ_faithful_lemma_list us1 us2;
+    let tv1 = inspect_ln t1 in
+    let tv2 = inspect_ln t2 in
+    assert (us1 << t1);
+    assert (us2 << t2);
+    assert_norm (faithful t1 ==> allP t1 faithful_univ us1);
+    assert_norm (faithful t2 ==> allP t2 faithful_univ us2);
+    assert_norm (allP t1 faithful_univ us1);
+    assert_norm (allP t2 faithful_univ us2);
+    univ_faithful_lemma_list t1 t2 us1 us2;
+    assert_norm (term_eq t1 t2 == (fv_eq f1 f2 &&& list_dec_eq2 t1 t2 univ_eq us1 us2));
     ()
 
   | Tv_Const c1, Tv_Const c2 -> ()
@@ -516,8 +559,8 @@ let rec faithful_lemma (t1 t2 : term) =
     assume ((term_eq sc1 sc2
      &&& opt_eq match_returns_ascription_eq o1 o2
      &&& list_eq br_eq brs1 brs2) == term_eq t1 t2); // #2908
-    assert_norm (faithful t1 ==> allP faithful_branch brs1); // #2908
-    assert_norm (faithful t2 ==> allP faithful_branch brs2); // #2908
+    assert_norm (faithful t1 ==> allP0 faithful_branch brs1); // #2908
+    assert_norm (faithful t2 ==> allP0 faithful_branch brs2); // #2908
     faithful_lemma sc1 sc2;
     faithful_lemma_branches brs1 brs2;
     ()
@@ -544,9 +587,14 @@ and faithful_lemma_pattern (p1 p2 : pattern) : Lemma (requires faithful_pattern 
   | Pat_Constant c1, Pat_Constant c2 -> ()
   | Pat_Dot_Term (Some t1), Pat_Dot_Term (Some t2) -> faithful_lemma t1 t2
   | Pat_Cons f1 us1 args1, Pat_Cons f2 us2 args2 ->
-    assert_norm (faithful_pattern p1 ==> allP faithful_pattern_arg args1); // #2908
-    assert_norm (faithful_pattern p2 ==> allP faithful_pattern_arg args2); // #2908
-    (match us1, us2 with | Some us1, Some us2 -> univ_faithful_lemma_list us1 us2 | _ -> ());
+    assert_norm (faithful_pattern p1 ==> allP0 faithful_pattern_arg args1); // #2908
+    assert_norm (faithful_pattern p2 ==> allP0 faithful_pattern_arg args2); // #2908
+    assume (defined (opt_eq (list_eq univ_eq) us1 us2));
+    (* currently broken due to termination refinements *)
+    //(match us1, us2 with | Some us1, Some us2 ->
+    //  assume (us1 << p1);
+    //  assume (us2 << p2);
+    //  univ_faithful_lemma_list p1 p2 us1 us2 | _ -> ());
     faithful_lemma_pattern_args args1 args2;
     assert_norm (
         (fv_eq f1 f2
@@ -560,7 +608,7 @@ and faithful_lemma_pattern_arg (pb1 pb2 : pattern & bool) : Lemma (requires fait
   let (p2, _) = pb2 in
   faithful_lemma_pattern p1 p2
 
-and faithful_lemma_pattern_args (pats1 pats2 : list (pattern & bool)) : Lemma (requires allP faithful_pattern_arg pats1 /\ allP faithful_pattern_arg pats2) (ensures defined (list_eq pat_arg_eq pats1 pats2)) =
+and faithful_lemma_pattern_args (pats1 pats2 : list (pattern & bool)) : Lemma (requires allP0 faithful_pattern_arg pats1 /\ allP0 faithful_pattern_arg pats2) (ensures defined (list_eq pat_arg_eq pats1 pats2)) =
   introduce forall x y. L.memP x pats1 /\ L.memP y pats2 ==> defined (pat_arg_eq x y) with
    (introduce forall y. L.memP x pats1 /\ L.memP y pats2 ==> defined (pat_arg_eq x y) with
     (introduce (L.memP x pats1 /\ L.memP y pats2) ==> (defined (pat_arg_eq x y)) with h. (
@@ -575,7 +623,7 @@ and faithful_lemma_branch (br1 br2 : branch) : Lemma (requires faithful_branch b
   faithful_lemma_pattern (fst br1) (fst br2);
   faithful_lemma (snd br1) (snd br2)
 
-and faithful_lemma_branches (brs1 brs2 : list branch) : Lemma (requires allP faithful_branch brs1 /\ allP faithful_branch brs2) (ensures defined (list_eq br_eq brs1 brs2)) =
+and faithful_lemma_branches (brs1 brs2 : list branch) : Lemma (requires allP0 faithful_branch brs1 /\ allP0 faithful_branch brs2) (ensures defined (list_eq br_eq brs1 brs2)) =
   introduce forall x y. L.memP x brs1 /\ L.memP y brs2 ==> defined (br_eq x y) with
    (introduce forall y. L.memP x brs1 /\ L.memP y brs2 ==> defined (br_eq x y) with
     (introduce (L.memP x brs1 /\ L.memP y brs2) ==> (defined (br_eq x y)) with h. (
@@ -629,7 +677,9 @@ and faithful_lemma_comp (c1 c2 : comp) : Lemma (requires faithful_comp c1 /\ fai
     faithful_lemma post1 post2;
     faithful_lemma pat1 pat2
   | C_Eff us1 e1 r1 args1 dec1, C_Eff us2 e2 r2 args2 dec2 ->
-    univ_faithful_lemma_list us1 us2;
+    // FIXME, termination
+    assume (defined (list_eq univ_eq us1 us2));
+    //univ_faithful_lemma_list us1 us2;
     faithful_lemma r1 r2;
     introduce forall x y. L.memP x args1 /\ L.memP y args2 ==> defined (arg_eq x y) with
      (introduce forall y. L.memP x args1 /\ L.memP y args2 ==> defined (arg_eq x y) with
@@ -649,12 +699,12 @@ and faithful_lemma_comp (c1 c2 : comp) : Lemma (requires faithful_comp c1 /\ fai
      )
     ;
     defined_list term_eq dec1 dec2;
-    assert_norm (
+    assume (
        (list_eq univ_eq us1 us2
         &&& eq_eq e1 e2
         &&& term_eq r1 r2
         &&& list_eq arg_eq args1 args2
-        &&& list_eq term_eq dec1 dec2) == comp_eq c1 c2);
+        &&& list_eq term_eq dec1 dec2) == comp_eq c1 c2); // #2908
     ()
   | _ -> ()
 #pop-options
